experiments with empty initial disk

core/Net.v
@@ -48,6 +48,11 @@ Class MultiParams (P : BaseParams) :=
     input_handlers : name -> input -> data -> (list output) * data * list (name * msg)
   }.
 
+Class FailureParams `(P : MultiParams) :=
+  {
+    reboot : data -> data
+  }.
+
 Class DiskMultiParams (P : BaseParams) :=
   {
     d_name : Type ;
@@ -66,12 +71,7 @@ Class DiskMultiParams (P : BaseParams) :=
 
 Class DiskFailureParams `(P : DiskMultiParams) :=
   {
-    d_reboot : disk -> option data
-  }.
-
-Class FailureParams `(P : MultiParams) :=
-  {
-    reboot : data -> data
+    d_reboot : d_name -> disk -> data
   }.
 
 Definition do_disk file_name :=
@@ -103,8 +103,9 @@ Class DiskOpMultiParams (P : BaseParams) :=
 
 Class DiskOpFailureParams `(P : DiskOpMultiParams) :=
   {
-    do_reboot : do_name -> (file_name -> IOStreamWriter.wire) ->
-                option (data * do_disk file_name)
+    do_reboot :
+      do_name -> (file_name -> IOStreamWriter.wire) ->
+      data * do_disk file_name
   }.
 
 Class NameOverlayParams `(P : MultiParams) :=
@@ -558,12 +559,11 @@ Section StepFailureDisk.
       step_failure_disk (failed, net) (failed, net') []
   | StepFailureDisk_fail :  forall h net failed,
       step_failure_disk (failed, net) (h :: failed, net) []
-  | StepFailureDisk_reboot : forall h net net' failed failed' d,
+  | StepFailureDisk_reboot : forall h net net' failed failed',
       In h failed ->
       failed' = remove d_name_eq_dec h failed ->
-      d_reboot (nwdDisk net h) = Some d ->
       net' = mkdNetwork (nwdPackets net)
-                        (update d_name_eq_dec (nwdState net) h d)
+                        (update d_name_eq_dec (nwdState net) h (d_reboot h (nwdDisk net h)))
                         (nwdDisk net) ->
       step_failure_disk (failed, net) (failed', net') [].
 
@@ -644,7 +644,7 @@ Section StepFailureDiskOp.
   | StepFailureDiskOp_reboot : forall h net net' failed failed' d dsk,
       In h failed ->
       failed' = remove do_name_eq_dec h failed ->
-      do_reboot h (disk_to_wire (nwdoDisk net h)) = Some (d, dsk) ->
+      do_reboot h (disk_to_wire (nwdoDisk net h)) = (d, dsk) ->
       net' = mkdoNetwork (nwdoPackets net)
                         (update do_name_eq_dec (nwdoState net) h d)
                         (update do_name_eq_dec (nwdoDisk net) h dsk) ->
