systems/Counter.v
@@ -27,59 +27,48 @@ Definition Output_eq_dec : forall x y : Output, {x = y} + {x <> y}.
   destruct x,y. auto.
 Defined.
 
-Definition Data := nat.
+Record Data := mkData { count : nat }.
 
-Definition init_Data := 0.
+Definition init_Data : Data := mkData 0.
 
-Definition Handler (S A : Type) := GenHandler (Name * Msg) S Output A.
+Definition Handler (S : Type) := GenHandler (Name * Msg) S Output unit.
 
-Definition disk := IOStreamWriter.wire.
-
-Definition snapshot : Handler Data disk :=
-  s <- get ;; ret (serialize_top (serialize s)).
-
-Definition reboot (s : IOStreamWriter.wire) : option Data :=
-  deserialize_top deserialize s.
-
-
-(* Definition keep_disk : Handler Data := *)
-Definition PrimaryNetHandler (m : Msg) : Handler Data unit :=
+Definition PrimaryNetHandler (m : Msg) : Handler Data :=
   match m with
   | ack => write_output inc_executed
   | _ => nop
   end.
 
-Definition PrimaryInputHandler (i : Input) : Handler Data unit :=
+Definition PrimaryInputHandler (i : Input) : Handler Data :=
   match i with
-  | request_inc => modify S ;; send (backup, inc)
+  | request_inc =>
+    st <- get ;;
+    put (mkData (S (count st))) ;;
+    send (backup, inc)
   end.
 
-Definition BackupNetHandler (m : Msg) : Handler Data unit :=
+Definition BackupNetHandler (m : Msg) : Handler Data :=
   match m with
-  | inc => modify S ;; send (primary, ack)
+  | inc =>
+    st <- get ;;
+    put (mkData (S (count st))) ;;
+    send (primary, ack)
   | _ => nop
   end.
 
-Definition BackupInputHandler (i : Input) : Handler Data unit := nop.
+Definition BackupInputHandler (i : Input) : Handler Data := nop.
 
-Definition NetHandler' (me : Name) (m : Msg) : Handler Data unit :=
+Definition NetHandler (me : Name) (m : Msg) : Handler Data :=
   match me with
   | primary => PrimaryNetHandler m
   | backup => BackupNetHandler m
   end.
 
-Definition NetHandler (me : Name) (m : Msg) : Handler Data disk :=
-  NetHandler' me m ;;
-              snapshot.
-
-Definition InputHandler' (me : Name) (i : Input) : Handler Data unit :=
+Definition InputHandler (me : Name) (i : Input) : Handler Data :=
   match me with
   | primary => PrimaryInputHandler i
   | backup => BackupInputHandler i
   end.
-
-Definition InputHandler (me : Name) (i : Input) : Handler Data disk :=
-  InputHandler' me i;; snapshot.
 
 Instance Counter_BaseParams : BaseParams :=
   {
@@ -100,7 +89,49 @@ Proof.
   repeat constructor; simpl; intuition discriminate.
 Qed.
 
-Instance Counter_MultiParams : DiskMultiParams Counter_BaseParams :=
+Import DeserializerNotations.
+
+Definition Data_serialize (d : Data) : IOStreamWriter.t :=
+  serialize x00 +$+ serialize (count d).
+
+Definition Data_deserialize : ByteListReader.t Data :=
+  tag <- deserialize ;;
+  match tag with
+  | x00 => mkData <$> deserialize
+  | _ => ByteListReader.error
+  end.
+
+Lemma Data_serialize_deserialize_id :
+  serialize_deserialize_id_spec Data_serialize Data_deserialize.
+Proof.
+  intros.
+  unfold Data_serialize, Data_deserialize.
+  destruct a.
+  repeat (cheerios_crush; simpl).
+Qed.
+
+Instance Data_Serializer : Serializer Data :=
+  {
+    serialize := Data_serialize;
+    deserialize := Data_deserialize;
+    serialize_deserialize_id := Data_serialize_deserialize_id
+  }.
+
+Definition disk_reboot (s : IOStreamWriter.wire) : Data := 
+  match deserialize_top deserialize s with
+  | Some d => d
+  | None => init_Data
+  end.
+
+Definition DiskNetHandler dst (src : Name) m st :=
+  let '(out, data, ps) := runGenHandler_ignore st (NetHandler dst m) in
+  (serialize_top (serialize data), out, data, ps).
+
+Definition DiskInputHandler h inp st :=
+  let '(out, data, ps) := runGenHandler_ignore st (InputHandler h inp) in
+  (serialize_top (serialize data), out, data, ps).
+
+Instance Counter_DiskMultiParams : DiskMultiParams Counter_BaseParams :=
   {
     d_name := Name;
     d_name_eq_dec := Name_eq_dec;
@@ -109,24 +140,27 @@ Instance Counter_MultiParams : DiskMultiParams Counter_BaseParams :=
     d_nodes := Nodes;
     d_all_names_nodes := all_Names_Nodes;
     d_no_dup_nodes := NoDup_Nodes;
+    disk := IOStreamWriter.wire;
     d_init_handlers := fun _ => init_Data;
-    d_init_disk := fun _ => (serialize_top (serialize 0));
-    d_net_handlers := fun dst src msg s => runGenHandler s (NetHandler dst msg);
-    d_input_handlers := fun nm i s => runGenHandler s (InputHandler nm i)
+    d_init_disk := fun _ => serialize_top IOStreamWriter.empty;
+    d_net_handlers := DiskNetHandler;
+    d_input_handlers := DiskInputHandler
   }.
 
-Instance Counter_FailureParams : DiskFailureParams Counter_MultiParams :=
+Instance Counter_FailureParams : DiskFailureParams Counter_DiskMultiParams :=
   {
-    d_reboot := reboot
+    d_reboot := fun _ => disk_reboot
   }.
 
+(*
 Lemma net_handlers_NetHandler :
   forall h src m d os d' ms dsk,
     d_net_handlers h src m d = (dsk, os, d', ms) ->
-    NetHandler h m d = (dsk, os, d', ms).
+    DiskNetHandler h src m d = (dsk, os, d', ms).
 Proof.
   intros.
   simpl in *.
+  unfold DiskNetHandler in *.
   monad_unfold.
   repeat break_let.
   auto.
@@ -143,13 +177,14 @@ Proof.
   repeat break_let.
   auto.
 Qed.
+*)
 
 Lemma PrimaryNetHandler_no_msgs :
   forall m d ms d' o u,
-    (PrimaryNetHandler m;; snapshot)  d = (u, o, d', ms) ->
+    PrimaryNetHandler m  d = (u, o, d', ms) ->
     ms = [].
 Proof.
-  unfold PrimaryNetHandler, snapshot.
+  unfold PrimaryNetHandler.
   intros. monad_unfold.
   repeat break_match; repeat find_inversion; auto.
 Qed.
@@ -193,9 +228,9 @@ Qed.
 Lemma InputHandler_inc_in_flight_to_backup_preserved :
   forall h i d u o d' l,
     InputHandler h i d = (u, o, d', l) ->
-    d' = d + inc_in_flight_to_backup (d_send_packets h l).
+    count d' = count d + inc_in_flight_to_backup (d_send_packets h l).
 Proof.
-  unfold InputHandler, InputHandler', PrimaryInputHandler, BackupInputHandler, snapshot.
+  unfold InputHandler, PrimaryInputHandler, BackupInputHandler.
   simpl.
   intros.
   monad_unfold.
@@ -206,14 +241,13 @@ Qed.
 Lemma NetHandler_inc_in_flight_to_backup_preserved :
   forall p d u o d' l,
     NetHandler (d_pDst p) (d_pBody p) d = (u, o, d', l) ->
-    d' + inc_in_flight_to_backup (d_send_packets (d_pDst p) l) = d + inc_in_flight_to_backup [p].
+    count d' + inc_in_flight_to_backup (d_send_packets (d_pDst p) l) = count d + inc_in_flight_to_backup [p].
 Proof.
-  unfold NetHandler, NetHandler', PrimaryNetHandler, BackupNetHandler.
+  unfold NetHandler, PrimaryNetHandler, BackupNetHandler.
   intros.
   monad_unfold.
   destruct p. simpl in *.
-  repeat break_match; repeat find_inversion; simpl; try rewrite inc_in_flight_to_backup_nil;
-  unfold Data in *; compute;
+  repeat break_match; repeat find_inversion; simpl; try rewrite inc_in_flight_to_backup_nil; compute;
   auto with *.
 Qed.
 
@@ -222,9 +256,9 @@ Lemma InputHandler_backup_no_msgs :
     InputHandler backup i d = (u, o, d', l) ->
     l = [].
 Proof.
-  simpl. unfold InputHandler, InputHandler', BackupInputHandler.
+  simpl. unfold InputHandler, BackupInputHandler.
   intros.
-  unfold snapshot in *. monad_unfold.
+  monad_unfold.
   find_inversion.
   auto.
 Qed.
@@ -237,13 +271,12 @@ Proof.
 Qed.
 
 
-
 Lemma backup_plus_network_eq_primary :
   forall net tr,
-    step_async_disk_star (params := Counter_MultiParams)
+    step_async_disk_star (params := Counter_DiskMultiParams)
                          step_async_disk_init
                          net tr -> 
-    nwdState net backup + inc_in_flight_to_backup (nwdPackets net) = nwdState net primary.
+    count (nwdState net backup) + inc_in_flight_to_backup (nwdPackets net) = count (nwdState net primary).
 Proof.
   intros.
   remember step_async_disk_init as y in *.
@@ -254,7 +287,13 @@ Proof.
     match goal with
     | [ H : step_async_disk _ _ _ |- _ ] => invc H
     end; simpl.
-    + find_apply_lem_hyp net_handlers_NetHandler.
+    + unfold d_net_handlers in *.
+      simpl in *.
+      unfold DiskNetHandler in *.
+      repeat break_let.
+      unfold runGenHandler_ignore in *.
+      repeat break_let.
+      repeat find_inversion.
       find_copy_apply_lem_hyp NetHandler_inc_in_flight_to_backup_preserved.
       repeat find_rewrite.
       rewrite cons_is_app in IHrefl_trans_1n_trace1.
@@ -271,22 +310,32 @@ Proof.
            try rewrite H0;
            assumption.
       * omega.
-    + find_apply_lem_hyp input_handlers_InputHandlers.
+    + unfold d_input_handlers in *.
+      simpl in *.
+      unfold DiskInputHandler in *.
+      repeat break_let.
+      unfold runGenHandler_ignore in *.
+      repeat break_let.
+      repeat find_inversion.
       find_copy_apply_lem_hyp InputHandler_inc_in_flight_to_backup_preserved.
-      unfold send_packets in *. simpl in *.
+      unfold d_send_packets in *. simpl in *.
       rewrite inc_in_flight_to_backup_app. subst.
       destruct h eqn:?;
                try rewrite update_same;
         try rewrite update_diff by congruence.
       * omega.
-      * erewrite InputHandler_backup_no_msgs with (l := l) by eauto.
-        simpl. rewrite inc_in_flight_to_backup_nil. omega.
+      * revert H0.
+        erewrite InputHandler_backup_no_msgs with (l := l) by eauto.
+        simpl.
+        rewrite inc_in_flight_to_backup_nil.
+        intros.
+        omega.
 Qed.
 
 Theorem primary_ge_backup :
   forall net tr,
-    step_async_disk_star (params := Counter_MultiParams) step_async_disk_init net tr ->
-    nwdState net backup <= nwdState net primary.
+    step_async_disk_star (params := Counter_DiskMultiParams) step_async_disk_init net tr ->
+    count (nwdState net backup) <= count (nwdState net primary).
 Proof.
   intros.
   apply backup_plus_network_eq_primary in H.
@@ -362,7 +411,7 @@ Lemma InputHandler_trace_preserved :
     inc_in_flight_to_backup (d_send_packets h l) +
     ack_in_flight_to_primary (d_send_packets h l).
 Proof.
-  unfold InputHandler, InputHandler', snapshot, PrimaryInputHandler, BackupInputHandler.
+  unfold InputHandler, PrimaryInputHandler, BackupInputHandler.
   simpl.
   intros.
   monad_unfold.
@@ -378,12 +427,12 @@ Lemma NetHandler_trace_preserved :
     inc_in_flight_to_backup (d_send_packets (d_pDst p) l) +
     ack_in_flight_to_primary (d_send_packets (d_pDst p) l).
 Proof.
-  unfold NetHandler, NetHandler', snapshot, PrimaryNetHandler, BackupNetHandler.
+  unfold NetHandler, PrimaryNetHandler, BackupNetHandler.
   intros.
   monad_unfold.
   destruct p. simpl in *.
   repeat break_match; repeat find_inversion; simpl; try rewrite inc_in_flight_to_backup_nil;
-  unfold Data in *; compute;
+  compute;
   auto with *.
 Qed.
 
@@ -414,7 +463,7 @@ Qed.
 
 Lemma inputs_eq_outputs_plus_inc_plus_ack :
   forall net tr,
-    step_async_disk_star (params := Counter_MultiParams) step_async_disk_init net tr ->
+    step_async_disk_star (params := Counter_DiskMultiParams) step_async_disk_init net tr ->
     trace_inputs tr = trace_outputs tr +
                       inc_in_flight_to_backup (nwdPackets net) +
                       ack_in_flight_to_primary (nwdPackets net).
@@ -428,7 +477,13 @@ Proof.
     match goal with
     | [ H : step_async_disk _ _ _ |- _ ] => invc H
     end; simpl.
-    + find_apply_lem_hyp net_handlers_NetHandler.
+    + unfold d_net_handlers in *.
+      simpl in *.
+      unfold DiskNetHandler in *.
+      repeat break_let.
+      unfold runGenHandler_ignore in *.
+      repeat break_let.
+      repeat find_inversion.
       repeat find_rewrite.
       rewrite trace_inputs_app.
       rewrite trace_outputs_app.
@@ -442,7 +497,13 @@ Proof.
       * rewrite ack_in_flight_to_primary_backup in * by auto.
         rewrite trace_outputs_backup in *. unfold send_packets in *.
         simpl in *. rewrite <- plus_n_O in *. omega.
-    + find_apply_lem_hyp input_handlers_InputHandlers.
+    + unfold d_input_handlers in *.
+      simpl in *.
+      unfold DiskInputHandler in *.
+      repeat break_let.
+      unfold runGenHandler_ignore in *.
+      repeat break_let.
+      repeat find_inversion.
       find_apply_lem_hyp InputHandler_trace_preserved.
       rewrite cons_is_app.
       repeat rewrite trace_inputs_app.
@@ -456,7 +517,7 @@ Qed.
 
 Theorem inputs_ge_outputs :
   forall net tr,
-    step_async_disk_star (params := Counter_MultiParams) step_async_disk_init net tr ->
+    step_async_disk_star (params := Counter_DiskMultiParams) step_async_disk_init net tr ->
     trace_outputs tr <= trace_inputs tr.
 Proof.
   intros.
@@ -465,90 +526,142 @@ Proof.
 Qed.
 
 Theorem net_handlers_reboot : forall node net p out d l dsk,
-    d_net_handlers node
-                   (d_pSrc p) (d_pBody p)
-                   (nwdState net node) = (dsk, out, d, l) ->
-      reboot (update Name_eq_dec (nwdDisk net) node dsk node) =
-  Some (update Name_eq_dec (nwdState net) node d node).
+    d_net_handlers node (d_pSrc p) (d_pBody p) (nwdState net node) = (dsk, out, d, l) ->
+    disk_reboot (update Name_eq_dec (nwdDisk net) node dsk node) =
+    update Name_eq_dec (nwdState net) node d node.
 Proof.
   intros.
   simpl in *.
-  destruct node;
-    unfold runGenHandler, NetHandler, NetHandler', PrimaryNetHandler, BackupNetHandler, snapshot in *;
-    monad_unfold;
-    repeat break_match;
-    repeat find_inversion;
-    apply serialize_deserialize_top_id.
+  destruct node; unfold DiskNetHandler, runGenHandler_ignore, NetHandler, PrimaryNetHandler, BackupNetHandler, disk_reboot in *.
+  - repeat break_let.
+    repeat break_match.
+    * repeat find_inversion.
+      update_destruct_max_simplify; try congruence.
+      pose proof (serialize_deserialize_top_id d).
+      unfold deserialize, serialize in H.
+      simpl in H.
+      find_rewrite.
+      find_injection.
+      reflexivity.
+    * repeat find_inversion.
+      update_destruct_max_simplify; try congruence.
+      pose proof (serialize_deserialize_top_id d).
+      unfold deserialize, serialize in H.
+      simpl in H.
+      find_rewrite.
+      find_injection.
+      reflexivity.
+    * repeat find_inversion.
+      update_destruct_max_simplify; try congruence.
+      pose proof (serialize_deserialize_top_id d).
+      unfold deserialize, serialize in H.
+      simpl in H.
+      congruence.
+    * repeat find_inversion.
+      update_destruct_max_simplify; try congruence.
+      pose proof (serialize_deserialize_top_id d).
+      unfold deserialize, serialize in H.
+      simpl in H.
+      find_rewrite.
+      congruence.
+   - repeat break_let.
+     repeat break_match.
+     * repeat find_inversion.
+       monad_unfold.
+       simpl in *.
+       find_injection.
+       update_destruct_max_simplify; try congruence.
+       pose proof (serialize_deserialize_top_id {| count := S (count (nwdState net backup)) |}).
+       unfold deserialize, serialize in H.
+       simpl in H.
+       find_rewrite.
+       find_injection.
+       reflexivity.
+     * repeat find_inversion.
+       update_destruct_max_simplify; try congruence.
+       pose proof (serialize_deserialize_top_id d).
+       unfold deserialize, serialize in H.
+       simpl in H.
+       find_rewrite.
+       find_inversion.
+       reflexivity.
+     * repeat find_inversion.
+       update_destruct_max_simplify; try congruence.
+       pose proof (serialize_deserialize_top_id d).
+       unfold deserialize, serialize in H.
+       simpl in H.
+       find_rewrite.
+       congruence.
+     * repeat find_inversion.
+       update_destruct_max_simplify; try congruence.
+       pose proof (serialize_deserialize_top_id d).
+       unfold deserialize, serialize in H.
+       simpl in H.
+       find_rewrite.
+       congruence.
 Qed.
 
 Theorem input_handlers_reboot : forall node net inp out d l dsk,
-    d_input_handlers node
-                     inp
-                   (nwdState net node) = (dsk, out, d, l) ->
-      reboot (update Name_eq_dec (nwdDisk net) node dsk node) =
-  Some (update Name_eq_dec (nwdState net) node d node).
+    d_input_handlers node inp (nwdState net node) = (dsk, out, d, l) ->
+      disk_reboot (update Name_eq_dec (nwdDisk net) node dsk node) =
+      update Name_eq_dec (nwdState net) node d node.
 Proof.
   intros.
   simpl in *.
-  destruct node;
-    unfold runGenHandler, InputHandler, InputHandler', PrimaryInputHandler, BackupInputHandler, snapshot in *;
-    monad_unfold;
+  destruct node; unfold DiskInputHandler, runGenHandler_ignore, InputHandler, PrimaryInputHandler, BackupInputHandler, disk_reboot in *.
+  monad_unfold;
+    repeat break_let;
     repeat break_match;
-    repeat find_inversion;
-    apply serialize_deserialize_top_id.
+    repeat find_inversion.
+  - update_destruct_max_simplify; try congruence.
+    pose proof (serialize_deserialize_top_id {| count := S (count (nwdState net primary)) |}).
+    unfold deserialize, serialize in H.
+    simpl in H.
+    find_rewrite.
+    find_injection.
+    reflexivity.
+  - update_destruct_max_simplify; try congruence.
+    pose proof (serialize_deserialize_top_id {| count := S (count (nwdState net primary)) |}).
+    simpl in H.
+    find_rewrite.
+    congruence.
+  - repeat break_let.
+    repeat find_inversion.
+    update_destruct_max_simplify; try congruence.
+    pose proof (serialize_deserialize_top_id d).
+    unfold deserialize, serialize in H.
+    simpl in H.
+    rewrite H.
+    reflexivity.
 Qed.
 
-Theorem disk_follows_local_state: forall net tr node,
-    step_async_disk_star (params := Counter_MultiParams) step_async_disk_init net tr ->
-    reboot (nwdDisk net node) = Some (nwdState net node).
+Theorem disk_follows_local_state: forall net tr h,
+    step_async_disk_star step_async_disk_init net tr ->
+    disk_reboot (nwdDisk net h) = nwdState net h.
 Proof.
   intros.
   remember step_async_disk_init as y in *.
   revert Heqy.
   induction H using refl_trans_1n_trace_n1_ind; intros; subst.
-  - simpl.
-    unfold init_Data.
-    apply serialize_deserialize_top_id.
+  - simpl.    
+    unfold init_Data, disk_reboot.
+    unfold deserialize_top, serialize_top; simpl.
+    rewrite IOStreamWriter.wire_wrap_unwrap.
+    rewrite IOStreamWriter.empty_unwrap.
+    unfold Data_deserialize.
+    cheerios_crush.
   - concludes.
     match goal with
     | [ H : step_async_disk _ _ _ |- _ ] => invc H
     end; simpl.
-    + destruct node, (d_pDst p).
-      * match goal with
-        | [H : d_net_handlers ?node _ _ _ = _ |- _] =>
-          apply (net_handlers_reboot node _ _ H)
-        end.
-      * rewrite update_diff.
-        -- rewrite update_diff.
-           ++ assumption.
-           ++ discriminate.
-        -- discriminate.
-      * rewrite update_diff.
-        -- rewrite update_diff.
-           ++ assumption.
-           ++ discriminate.
-        -- discriminate.
-      * match goal with
-        | [H : d_net_handlers ?node _ _ _ = _ |- _] =>
-          apply (net_handlers_reboot node _ _ H)
-        end.
-    + destruct node, h.
-      * match goal with
-        | [H : d_input_handlers ?node _ _ = _ |- _] =>
-          apply (input_handlers_reboot node _ _ H)
-        end.
-      * rewrite update_diff.
-        -- rewrite update_diff.
-           ++ assumption.
-           ++ discriminate.
-        -- discriminate.
-      * rewrite update_diff.
-        -- rewrite update_diff.
-           ++ assumption.
-           ++ discriminate.
-        -- discriminate.
-      * match goal with
-        | [H : d_input_handlers ?node _ _ = _ |- _] =>
-          apply (input_handlers_reboot node _ _ H)
-        end.
+    + match goal with
+      | [H : d_net_handlers _ _ _ _ = _ |- _] =>
+        apply net_handlers_reboot in H
+      end.
+      update_destruct_max_simplify; auto.
+    + match goal with
+      | [H : d_input_handlers ?node _ _ = _ |- _] =>
+        apply input_handlers_reboot in H
+      end.
+      update_destruct_max_simplify; auto.
 Qed.
